all before subst_principle... yet another scheme for avar_f that makes it easier to do subst

dev/lf/dot_rec.v
@@ -17,16 +17,16 @@ Inductive label: Set :=
 | label_typ: typ_label -> label
 | label_trm: trm_label -> label.
 
-Inductive bound_in : Set :=
-| in_sto : bound_in
-| in_ctx : bound_in.
+Inductive fvar : Set :=
+| in_sto : var -> fvar
+| in_ctx : var -> fvar.
 
 Inductive avar : Set :=
   | avar_b : nat -> avar
-  | avar_f : bound_in -> var -> avar.
+  | avar_f : fvar -> avar.
 
-Definition avar_s x := avar_f in_sto x.
-Definition avar_c x := avar_f in_ctx x.
+Definition avar_s x := avar_f (in_sto x).
+Definition avar_c x := avar_f (in_ctx x).
 
 Inductive typ : Set :=
   | typ_top  : typ
@@ -90,13 +90,13 @@ Definition defs_hasnt(ds: defs)(l: label) := get_def l ds = None.
 (** Opening replaces in some syntax a bound variable with dangling index (k)
    by a free variable x. *)
 
-Definition open_rec_avar (k: nat) (u: avar) (a: avar) : avar :=
+Definition open_rec_avar (k: nat) (u: fvar) (a: avar) : avar :=
   match a with
-  | avar_b i => If k = i then u else avar_b i
-  | avar_f b x => avar_f b x
+  | avar_b i => If k = i then avar_f u else avar_b i
+  | avar_f v => avar_f v
   end.
 
-Fixpoint open_rec_typ (k: nat) (u: avar) (T: typ): typ :=
+Fixpoint open_rec_typ (k: nat) (u: fvar) (T: typ): typ :=
   match T with
   | typ_top        => typ_top
   | typ_bot        => typ_bot
@@ -106,13 +106,13 @@ Fixpoint open_rec_typ (k: nat) (u: avar) (T: typ): typ :=
   | typ_bnd T      => typ_bnd (open_rec_typ (S k) u T)
   | typ_all T1 T2  => typ_all (open_rec_typ k u T1) (open_rec_typ (S k) u T2)
   end
-with open_rec_dec (k: nat) (u: avar) (D: dec): dec :=
+with open_rec_dec (k: nat) (u: fvar) (D: dec): dec :=
   match D with
   | dec_typ L T U => dec_typ L (open_rec_typ k u T) (open_rec_typ k u U)
   | dec_trm m T => dec_trm m (open_rec_typ k u T)
   end.
 
-Fixpoint open_rec_trm (k: nat) (u: avar) (t: trm): trm :=
+Fixpoint open_rec_trm (k: nat) (u: fvar) (t: trm): trm :=
   match t with
   | trm_var a      => trm_var (open_rec_avar k u a)
   | trm_val v      => trm_val (open_rec_val k u v)
@@ -120,17 +120,17 @@ Fixpoint open_rec_trm (k: nat) (u: avar) (t: trm): trm :=
   | trm_app f a    => trm_app (open_rec_avar k u f) (open_rec_avar k u a)
   | trm_let t1 t2  => trm_let (open_rec_trm k u t1) (open_rec_trm (S k) u t2)
   end
-with open_rec_val (k: nat) (u: avar) (v: val): val :=
+with open_rec_val (k: nat) (u: fvar) (v: val): val :=
   match v with
   | val_new T ds => val_new (open_rec_typ (S k) u T) (open_rec_defs (S k) u ds)
   | val_lambda T e => val_lambda (open_rec_typ k u T) (open_rec_trm (S k) u e)
   end
-with open_rec_def (k: nat) (u: avar) (d: def): def :=
+with open_rec_def (k: nat) (u: fvar) (d: def): def :=
   match d with
   | def_typ L T => def_typ L (open_rec_typ k u T)
   | def_trm m e => def_trm m (open_rec_trm k u e)
   end
-with open_rec_defs (k: nat) (u: avar) (ds: defs): defs :=
+with open_rec_defs (k: nat) (u: fvar) (ds: defs): defs :=
   match ds with
   | defs_nil => defs_nil
   | defs_cons tl d => defs_cons (open_rec_defs k u tl) (open_rec_def k u d)
@@ -147,10 +147,16 @@ Definition open_defs u l := open_rec_defs  0 u l.
 (* ###################################################################### *)
 (** ** Free variables *)
 
+Definition fv_fvar (v: fvar) : vars :=
+  match v with
+  | in_sto x => \{x}
+  | in_ctx x => \{x}
+  end.
+
 Definition fv_avar (a: avar) : vars :=
   match a with
   | avar_b i => \{}
-  | avar_f b x => \{x}
+  | avar_f v => fv_fvar v
   end.
 
 Fixpoint fv_typ (T: typ) : vars :=
@@ -201,16 +207,16 @@ Definition fv_ctx_types(G: ctx): vars := (fv_in_values (fun T => fv_typ T) G).
 Inductive red : trm -> sto -> trm -> sto -> Prop :=
 | red_sel : forall x m s t T ds,
     binds x (val_new T ds) s ->
-    defs_has (open_defs (avar_s x) ds) (def_trm m t) ->
+    defs_has (open_defs (in_sto x) ds) (def_trm m t) ->
     red (trm_sel (avar_s x) m) s t s
 | red_app : forall f a s T t,
     binds f (val_lambda T t) s ->
-    red (trm_app (avar_s f) (avar_s a)) s (open_trm (avar_s a) t) s
+    red (trm_app (avar_s f) (avar_s a)) s (open_trm (in_sto a) t) s
 | red_let : forall v t s x,
     x # s ->
-    red (trm_let (trm_val v) t) s (open_trm (avar_s x) t) (s & x ~ v)
+    red (trm_let (trm_val v) t) s (open_trm (in_sto x) t) (s & x ~ v)
 | red_let_var : forall t s x,
-    red (trm_let (trm_var (avar_s x)) t) s (open_trm (avar_s x) t) s
+    red (trm_let (trm_var (avar_s x)) t) s (open_trm (in_sto x) t) s
 | red_let_tgt : forall t0 t s t0' s',
     red t0 s t0' s' ->
     red (trm_let t0 t) s (trm_let t0' t) s'.
@@ -235,36 +241,36 @@ Inductive ty_trm : tymode -> sto -> ctx -> trm -> typ -> Prop :=
     ty_trm m s G (trm_var (avar_c x)) T
 | ty_all_intro : forall L m s G T t U,
     (forall x, x \notin L ->
-      ty_trm ty_general s (G & x ~ T) (open_trm (avar_c x) t) (open_typ (avar_c x) U)) ->
+      ty_trm ty_general s (G & x ~ T) (open_trm (in_ctx x) t) (open_typ (in_ctx x) U)) ->
     ty_trm m s G (trm_val (val_lambda T t)) (typ_all T U)
-| ty_all_elim : forall s G bx x bz z S T,
-    ty_trm ty_general s G (trm_var (avar_f bx x)) (typ_all S T) ->
-    ty_trm ty_general s G (trm_var (avar_f bz z)) S ->
-    ty_trm ty_general s G (trm_app (avar_f bx x) (avar_f bz z)) (open_typ (avar_f bz z) T)
+| ty_all_elim : forall s G x z S T,
+    ty_trm ty_general s G (trm_var (avar_f x)) (typ_all S T) ->
+    ty_trm ty_general s G (trm_var (avar_f z)) S ->
+    ty_trm ty_general s G (trm_app (avar_f x) (avar_f z)) (open_typ z T)
 | ty_new_intro : forall L m s G T ds,
     (forall x, x \notin L ->
-      ty_defs s (G & (x ~ open_typ (avar_c x) T)) (open_defs (avar_c x) ds) (open_typ (avar_c x) T)) ->
+      ty_defs s (G & (x ~ open_typ (in_ctx x) T)) (open_defs (in_ctx x) ds) (open_typ (in_ctx x) T)) ->
     ty_trm m s G (trm_val (val_new T ds)) (typ_bnd T)
-| ty_new_elim : forall s G bx x m T,
-    ty_trm ty_general s G (trm_var (avar_f bx x)) (typ_rcd (dec_trm m T)) ->
-    ty_trm ty_general s G (trm_sel (avar_f bx x) m) T
+| ty_new_elim : forall s G x m T,
+    ty_trm ty_general s G (trm_var (avar_f x)) (typ_rcd (dec_trm m T)) ->
+    ty_trm ty_general s G (trm_sel (avar_f x) m) T
 | ty_let : forall L s G t u T U,
     ty_trm ty_general s G t T ->
     (forall x, x \notin L ->
-      ty_trm ty_general s (G & x ~ T) (open_trm (avar_c x) u) U) ->
+      ty_trm ty_general s (G & x ~ T) (open_trm (in_ctx x) u) U) ->
     ty_trm ty_general s G (trm_let t u) U
-| ty_rec_intro : forall s G bx x T,
-    ty_trm ty_general s G (trm_var (avar_f bx x)) (open_typ (avar_f bx x) T) ->
-    ty_trm ty_general s G (trm_var (avar_f bx x)) (typ_bnd T)
-| ty_rec_elim : forall m s G bx x T,
-    ty_trm m s G (trm_var (avar_f bx x)) (typ_bnd T) ->
-    ty_trm m s G (trm_var (avar_f bx x)) (open_typ (avar_f bx x) T)
-| ty_and_intro : forall s G bx x T U,
-    ty_trm ty_general s G (trm_var (avar_f bx x)) T ->
-    ty_trm ty_general s G (trm_var (avar_f bx x)) U ->
-    ty_trm ty_general s G (trm_var (avar_f bx x)) (typ_and T U)
+| ty_rec_intro : forall s G x T,
+    ty_trm ty_general s G (trm_var (avar_f x)) (open_typ x T) ->
+    ty_trm ty_general s G (trm_var (avar_f x)) (typ_bnd T)
+| ty_rec_elim : forall m s G x T,
+    ty_trm m s G (trm_var (avar_f x)) (typ_bnd T) ->
+    ty_trm m s G (trm_var (avar_f x)) (open_typ x T)
+| ty_and_intro : forall s G x T U,
+    ty_trm ty_general s G (trm_var (avar_f x)) T ->
+    ty_trm ty_general s G (trm_var (avar_f x)) U ->
+    ty_trm ty_general s G (trm_var (avar_f x)) (typ_and T U)
 | ty_sub : forall m s G t T U,
-    (m = ty_precise -> exists b x, t = trm_var (avar_f b x)) ->
+    (m = ty_precise -> exists x, t = trm_var (avar_f x)) ->
     ty_trm m s G t T ->
     subtyp m s G T U ->
     ty_trm m s G t U
@@ -320,20 +326,20 @@ with subtyp : tymode -> sto -> ctx -> typ -> typ -> Prop :=
     subtyp ty_general s G (typ_sel (avar_c x) A) T
 | subtyp_sel2_tight: forall s G x A S ds T,
     binds x (val_new S ds) s ->
-    defs_has (open_defs (avar_s x) ds) (def_typ A T) ->
+    defs_has (open_defs (in_sto x) ds) (def_typ A T) ->
     subtyp ty_general s G T (typ_sel (avar_s x) A)
 | subtyp_sel1_tight: forall s G x A S ds T,
     binds x (val_new S ds) s ->
-    defs_has (open_defs (avar_s x) ds) (def_typ A T) ->
+    defs_has (open_defs (in_sto x) ds) (def_typ A T) ->
     subtyp ty_general s G (typ_sel (avar_s x) A) T
 | subtyp_all: forall L s G S1 T1 S2 T2,
     subtyp ty_general s G S2 S1 ->
     (forall x, x \notin L ->
-       subtyp ty_general s (G & x ~ S2) (open_typ (avar_c x) T1) (open_typ (avar_c x) T2)) ->
+       subtyp ty_general s (G & x ~ S2) (open_typ (in_ctx x) T1) (open_typ (in_ctx x) T2)) ->
     subtyp ty_general s G (typ_all S1 T1) (typ_all S2 T2)
 | subtyp_bnd: forall L s G T1 T2,
     (forall x, x \notin L ->
-       subtyp ty_general s (G & x ~ (typ_bnd T1)) (open_typ (avar_c x) T1) (open_typ (avar_c x) T2)) ->
+       subtyp ty_general s (G & x ~ (typ_bnd T1)) (open_typ (in_ctx x) T1) (open_typ (in_ctx x) T2)) ->
     subtyp ty_general s G (typ_bnd T1) (typ_bnd T2).
 
 Inductive wf_sto: ctx -> sto -> Prop :=
@@ -576,7 +582,7 @@ Proof.
     apply* H.
   + intros. subst.
     apply_fresh ty_new_intro as z; assert (zL: z \notin L) by auto.
-    - specialize (H z zL G1 G2 (G3 & z ~ open_typ (avar_c z) T)).
+    - specialize (H z zL G1 G2 (G3 & z ~ open_typ (in_ctx z) T)).
       repeat rewrite concat_assoc in H.
       apply* H.
   + intros. subst.
@@ -863,14 +869,19 @@ Qed.
 (* ###################################################################### *)
 (** ** Substitution *)
 
-Definition subst_avar (z: var) (u: avar) (a: avar) : avar :=
-  match a with
-  | avar_b i => avar_b i
-  | avar_f in_ctx x => avar_c x
-  | avar_f in_sto x => (If x = z then u else avar_s x)
+Definition subst_fvar (z: var) (u: fvar) (v: fvar) : fvar :=
+  match v with
+  | in_sto x => in_sto x
+  | in_ctx x => (If x = z then u else in_ctx x)
   end.
 
-Fixpoint subst_typ (z: var) (u: avar) (T: typ) { struct T } : typ :=
+Definition subst_avar (z: var) (u: fvar) (a: avar) : avar :=
+  match a with
+  | avar_b i => avar_b i
+  | avar_f v => avar_f (subst_fvar z u v)
+  end.
+
+Fixpoint subst_typ (z: var) (u: fvar) (T: typ) { struct T } : typ :=
   match T with
   | typ_top        => typ_top
   | typ_bot        => typ_bot
@@ -880,13 +891,13 @@ Fixpoint subst_typ (z: var) (u: avar) (T: typ) { struct T } : typ :=
   | typ_bnd T      => typ_bnd (subst_typ z u T)
   | typ_all T U    => typ_all (subst_typ z u T) (subst_typ z u U)
   end
-with subst_dec (z: var) (u: avar) (D: dec) { struct D } : dec :=
+with subst_dec (z: var) (u: fvar) (D: dec) { struct D } : dec :=
   match D with
   | dec_typ L T U => dec_typ L (subst_typ z u T) (subst_typ z u U)
   | dec_trm L U => dec_trm L (subst_typ z u U)
   end.
 
-Fixpoint subst_trm (z: var) (u: avar) (t: trm) : trm :=
+Fixpoint subst_trm (z: var) (u: fvar) (t: trm) : trm :=
   match t with
   | trm_var x        => trm_var (subst_avar z u x)
   | trm_val v        => trm_val (subst_val z u v)
@@ -894,31 +905,37 @@ Fixpoint subst_trm (z: var) (u: avar) (t: trm) : trm :=
   | trm_app x1 x2    => trm_app (subst_avar z u x1) (subst_avar z u x2)
   | trm_let t1 t2    => trm_let (subst_trm z u t1) (subst_trm z u t2)
   end
-with subst_val (z: var) (u: avar) (v: val) : val :=
+with subst_val (z: var) (u: fvar) (v: val) : val :=
   match v with
   | val_new T ds     => val_new (subst_typ z u T) (subst_defs z u ds)
   | val_lambda T t   => val_lambda (subst_typ z u T) (subst_trm z u t)
   end
-with subst_def (z: var) (u: avar) (d: def) : def :=
+with subst_def (z: var) (u: fvar) (d: def) : def :=
   match d with
   | def_typ L T => def_typ L (subst_typ z u T)
   | def_trm L t => def_trm L (subst_trm z u t)
   end
-with subst_defs (z: var) (u: avar) (ds: defs) : defs :=
+with subst_defs (z: var) (u: fvar) (ds: defs) : defs :=
   match ds with
   | defs_nil => defs_nil
   | defs_cons rest d => defs_cons (subst_defs z u rest) (subst_def z u d)
   end.
 
-Definition subst_ctx (z: var) (u: avar) (G: ctx) : ctx := map (subst_typ z u) G.
+Definition subst_ctx (z: var) (u: fvar) (G: ctx) : ctx := map (subst_typ z u) G.
 
 (* ###################################################################### *)
 (** ** Lemmas for var-by-var substitution *)
 
+Lemma subst_fresh_fvar: forall x y,
+  (forall v: fvar, x \notin fv_fvar v -> subst_fvar x y v = v).
+Proof.
+  intros. destruct* v. simpl. case_var*. simpls. notin_false.
+Qed.
+
 Lemma subst_fresh_avar: forall x y,
   (forall a: avar, x \notin fv_avar a -> subst_avar x y a = a).
 Proof.
-  intros. destruct* a. destruct* b. simpl. case_var*. simpls. notin_false.
+  intros. destruct* a. simpl. f_equal. apply* subst_fresh_fvar.
 Qed.
 
 Lemma subst_fresh_typ_dec: forall x y,
@@ -974,82 +991,73 @@ Proof.
     reflexivity.
 Qed.
 
-Lemma subst_open_commute_avar: forall x y u b yv,
-  y = avar_f b yv ->
+Lemma subst_open_commute_avar: forall x y u,
   (forall a: avar, forall n: Datatypes.nat,
     subst_avar x y (open_rec_avar n u a)
-    = open_rec_avar n (subst_avar x y u) (subst_avar  x y a)).
+    = open_rec_avar n (subst_fvar x y u) (subst_avar x y a)).
 Proof.
-  intros. unfold subst_avar, open_avar, open_rec_avar. destruct a.
+  intros. unfold subst_fvar, subst_avar, open_avar, open_rec_avar. destruct a.
   + repeat case_if; auto.
-  + subst. destruct b0. case_var*. unfold avar_c. reflexivity.
+  + reflexivity.
 Qed.
 
 (* "open and then substitute" = "substitute and then open" *)
-Lemma subst_open_commute_typ_dec: forall x y u b yv,
-  y = avar_f b yv ->
+Lemma subst_open_commute_typ_dec: forall x y u,
   (forall t : typ, forall n: nat,
      subst_typ x y (open_rec_typ n u t)
-     = open_rec_typ n (subst_avar x y u) (subst_typ x y t)) /\
+     = open_rec_typ n (subst_fvar x y u) (subst_typ x y t)) /\
   (forall D : dec, forall n: nat,
      subst_dec x y (open_rec_dec n u D)
-     = open_rec_dec n (subst_avar x y u) (subst_dec x y D)).
+     = open_rec_dec n (subst_fvar x y u) (subst_dec x y D)).
 Proof.
-  intros. apply typ_mutind; intros; simpl; f_equal*.
-  eapply subst_open_commute_avar; eauto.
+  intros. apply typ_mutind; intros; simpl; f_equal*. apply subst_open_commute_avar.
 Qed.
 
-Lemma subst_open_commute_typ: forall x y u T b yv,
-  y = avar_f b yv ->
-  subst_typ x y (open_typ u T) = open_typ (subst_avar x y u) (subst_typ x y T).
+Lemma subst_open_commute_typ: forall x y u T,
+  subst_typ x y (open_typ u T) = open_typ (subst_fvar x y u) (subst_typ x y T).
 Proof.
   intros. apply* subst_open_commute_typ_dec.
 Qed.
 
-Lemma subst_open_commute_dec: forall x y u D b yv,
-  y = avar_f b yv ->
-  subst_dec x y (open_dec u D) = open_dec (subst_avar x y u) (subst_dec x y D).
+Lemma subst_open_commute_dec: forall x y u D,
+  subst_dec x y (open_dec u D) = open_dec (subst_fvar x y u) (subst_dec x y D).
 Proof.
   intros. apply* subst_open_commute_typ_dec.
 Qed.
 
 (* "open and then substitute" = "substitute and then open" *)
-Lemma subst_open_commute_trm_val_def_defs: forall x y u b yv,
-  y = avar_f b yv ->
+Lemma subst_open_commute_trm_val_def_defs: forall x y u,
   (forall t : trm, forall n: Datatypes.nat,
      subst_trm x y (open_rec_trm n u t)
-     = open_rec_trm n (subst_avar x y u) (subst_trm x y t)) /\
+     = open_rec_trm n (subst_fvar x y u) (subst_trm x y t)) /\
   (forall v : val, forall n: Datatypes.nat,
      subst_val x y (open_rec_val n u v)
-     = open_rec_val n (subst_avar x y u) (subst_val x y v)) /\
+     = open_rec_val n (subst_fvar x y u) (subst_val x y v)) /\
   (forall d : def , forall n: Datatypes.nat,
      subst_def x y (open_rec_def n u d)
-     = open_rec_def n (subst_avar x y u) (subst_def x y d)) /\
+     = open_rec_def n (subst_fvar x y u) (subst_def x y d)) /\
   (forall ds: defs, forall n: Datatypes.nat,
      subst_defs x y (open_rec_defs n u ds)
-     = open_rec_defs n (subst_avar x y u) (subst_defs x y ds)).
+     = open_rec_defs n (subst_fvar x y u) (subst_defs x y ds)).
 Proof.
   intros. apply trm_mutind; intros; simpl; f_equal*;
     (apply* subst_open_commute_avar || apply* subst_open_commute_typ_dec).
 Qed.
 
-Lemma subst_open_commute_trm: forall x y u t b yv,
-  y = avar_f b yv ->
-  subst_trm x y (open_trm u t) = open_trm (subst_avar x y u) (subst_trm x y t).
+Lemma subst_open_commute_trm: forall x y u t,
+  subst_trm x y (open_trm u t) = open_trm (subst_fvar x y u) (subst_trm x y t).
 Proof.
   intros. apply* subst_open_commute_trm_val_def_defs.
 Qed.
 
-Lemma subst_open_commute_val: forall x y u v b yv,
-  y = avar_f b yv ->
-  subst_val x y (open_val u v) = open_val (subst_avar x y u) (subst_val x y v).
+Lemma subst_open_commute_val: forall x y u v,
+  subst_val x y (open_val u v) = open_val (subst_fvar x y u) (subst_val x y v).
 Proof.
   intros. apply* subst_open_commute_trm_val_def_defs.
 Qed.
 
-Lemma subst_open_commute_defs: forall x y u ds b yv,
-  y = avar_f b yv ->
-  subst_defs x y (open_defs u ds) = open_defs (subst_avar x y u) (subst_defs x y ds).
+Lemma subst_open_commute_defs: forall x y u ds,
+  subst_defs x y (open_defs u ds) = open_defs (subst_fvar x y u) (subst_defs x y ds).
 Proof.
   intros. apply* subst_open_commute_trm_val_def_defs.
 Qed.
@@ -1057,7 +1065,7 @@ Qed.
 (* "Introduce a substitution after open": Opening a term t with a var u is the
    same as opening t with x and then replacing x by u. *)
 Lemma subst_intro_trm: forall x u t, x \notin (fv_trm t) ->
-  open_trm u t = subst_trm x u (open_trm x t).
+  open_trm u t = subst_trm x u (open_trm (in_ctx x) t).
 Proof.
   introv Fr. unfold open_trm. rewrite* subst_open_commute_trm.
   destruct (@subst_fresh_trm_val_def_defs x u) as [Q _]. rewrite* (Q t).
@@ -1065,7 +1073,7 @@ Proof.
 Qed.
 
 Lemma subst_intro_val: forall x u v, x \notin (fv_val v) ->
-  open_val u v = subst_val x u (open_val x v).
+  open_val u v = subst_val x u (open_val (in_ctx x) v).
 Proof.
   introv Fr. unfold open_trm. rewrite* subst_open_commute_val.
   destruct (@subst_fresh_trm_val_def_defs x u) as [_ [Q _]]. rewrite* (Q v).
@@ -1073,7 +1081,7 @@ Proof.
 Qed.
 
 Lemma subst_intro_defs: forall x u ds, x \notin (fv_defs ds) ->
-  open_defs u ds = subst_defs x u (open_defs x ds).
+  open_defs u ds = subst_defs x u (open_defs (in_ctx x) ds).
 Proof.
   introv Fr. unfold open_trm. rewrite* subst_open_commute_defs.
   destruct (@subst_fresh_trm_val_def_defs x u) as [_ [_ [_ Q]]]. rewrite* (Q ds).
@@ -1081,7 +1089,7 @@ Proof.
 Qed.
 
 Lemma subst_intro_typ: forall x u T, x \notin (fv_typ T) ->
-  open_typ u T = subst_typ x u (open_typ x T).
+  open_typ u T = subst_typ x u (open_typ (in_ctx x) T).
 Proof.
   introv Fr. unfold open_typ. rewrite* subst_open_commute_typ.
   destruct (@subst_fresh_typ_dec x u) as [Q _]. rewrite* (Q T).
@@ -1089,24 +1097,32 @@ Proof.
 Qed.
 
 Lemma subst_intro_dec: forall x u D, x \notin (fv_dec D) ->
-  open_dec u D = subst_dec x u (open_dec x D).
+  open_dec u D = subst_dec x u (open_dec (in_ctx x) D).
 Proof.
   introv Fr. unfold open_trm. rewrite* subst_open_commute_dec.
   destruct (@subst_fresh_typ_dec x u) as [_ Q]. rewrite* (Q D).
   unfold subst_fvar. case_var*.
 Qed.
 
-Lemma subst_undo_avar: forall x y,
-  (forall a, y \notin fv_avar a -> (subst_avar y x (subst_avar x y a)) = a).
+Lemma subst_undo_fvar: forall x y,
+  (forall v, y \notin fv_fvar v -> (subst_fvar y (in_ctx x) (subst_fvar x (in_ctx y) v)) = v).
 Proof.
-  intros. unfold subst_avar, subst_fvar, open_avar, open_rec_avar; destruct a.
+  intros. unfold subst_fvar, subst_fvar; destruct v.
   + reflexivity.
-  + unfold fv_avar in H. assert (y <> v) by auto. repeat case_if; reflexivity.
+  + unfold fv_fvar in H. assert (y <> v) by auto. repeat case_if; reflexivity.
+Qed.
+
+Lemma subst_undo_avar: forall x y,
+  (forall a, y \notin fv_avar a -> (subst_avar y (in_ctx x) (subst_avar x (in_ctx y) a)) = a).
+Proof.
+  intros. unfold subst_avar; destruct a.
+  + reflexivity.
+  + f_equal. apply* subst_undo_fvar.
 Qed.
 
 Lemma subst_undo_typ_dec: forall x y,
-   (forall T , y \notin fv_typ  T  -> (subst_typ  y x (subst_typ  x y T )) = T )
-/\ (forall D , y \notin fv_dec  D  -> (subst_dec  y x (subst_dec  x y D )) = D ).
+   (forall T , y \notin fv_typ  T  -> (subst_typ y (in_ctx x) (subst_typ  x (in_ctx y) T )) = T )
+/\ (forall D , y \notin fv_dec  D  -> (subst_dec y (in_ctx x) (subst_dec  x (in_ctx y) D )) = D ).
 Proof.
   intros.
   apply typ_mutind; intros; simpl; unfold fv_typ, fv_dec in *; f_equal*.
@@ -1114,10 +1130,10 @@ Proof.
 Qed.
 
 Lemma subst_undo_trm_val_def_defs: forall x y,
-   (forall t , y \notin fv_trm  t  -> (subst_trm  y x (subst_trm  x y t )) = t )
-/\ (forall v , y \notin fv_val  v  -> (subst_val  y x (subst_val  x y v )) = v )
-/\ (forall d , y \notin fv_def  d  -> (subst_def  y x (subst_def  x y d )) = d )
-/\ (forall ds, y \notin fv_defs ds -> (subst_defs y x (subst_defs x y ds)) = ds).
+   (forall t , y \notin fv_trm  t  -> (subst_trm  y (in_ctx x) (subst_trm  x (in_ctx y) t )) = t )
+/\ (forall v , y \notin fv_val  v  -> (subst_val  y (in_ctx x) (subst_val  x (in_ctx y) v )) = v )
+/\ (forall d , y \notin fv_def  d  -> (subst_def  y (in_ctx x) (subst_def  x (in_ctx y) d )) = d )
+/\ (forall ds, y \notin fv_defs ds -> (subst_defs y (in_ctx x) (subst_defs x (in_ctx y) ds)) = ds).
 Proof.
   intros.
   apply trm_mutind; intros; simpl; unfold fv_trm, fv_val, fv_def, fv_defs in *; f_equal*;
@@ -1125,23 +1141,31 @@ Proof.
 Qed.
 
 Lemma subst_typ_undo: forall x y T,
-  y \notin fv_typ T -> (subst_typ y x (subst_typ x y T)) = T.
+  y \notin fv_typ T -> (subst_typ y (in_ctx x) (subst_typ x (in_ctx y) T)) = T.
 Proof.
   apply* subst_undo_typ_dec.
 Qed.
 
 Lemma subst_trm_undo: forall x y t,
-  y \notin fv_trm t -> (subst_trm y x (subst_trm x y t)) = t.
+  y \notin fv_trm t -> (subst_trm y (in_ctx x) (subst_trm x (in_ctx y) t)) = t.
 Proof.
   apply* subst_undo_trm_val_def_defs.
+Qed.
+
+Lemma subst_idempotent_fvar: forall x y,
+  (forall v, (subst_fvar x y (subst_fvar x y v)) = (subst_fvar x y v)).
+Proof.
+  intros. unfold subst_fvar; destruct v.
+  + reflexivity.
+  + case_if; eauto; destruct y; eauto; case_if; eauto.
 Qed.
 
 Lemma subst_idempotent_avar: forall x y,
   (forall a, (subst_avar x y (subst_avar x y a)) = (subst_avar x y a)).
 Proof.
-  intros. unfold subst_avar, subst_fvar, open_avar, open_rec_avar; destruct a.
+  intros. unfold subst_avar; destruct a.
   + reflexivity.
-  + repeat case_if; reflexivity.
+  + f_equal. apply* subst_idempotent_fvar.
 Qed.
 
 Lemma subst_idempotent_typ_dec: forall x y,
